blah

coq/wfrec.v
@@ -3,41 +3,79 @@ From Coq Require Import Arith Lia.
 Section Acc.
   Variables (X: Type) (R: X -> X -> Prop).
   Inductive Acc (x: X) : Prop := AccC (h: forall y, R y x -> Acc y).
-  Definition wf := forall x, Acc x.
-  Variable alpha: wf.
-  Variable (p: X -> Type).
+  Fact Acc_iff x :
+    Acc x <-> forall y, R y x -> Acc y.
+  Proof.
+    split.
+    - intros [h]. exact h.
+    - apply AccC.
+  Qed.
+  Variable p: X -> Type.
   Variable F: (forall x, (forall y, R y x -> p y) -> p x).
   Definition W'
     : forall x, Acc x -> p x
     := fix f x a :=
          match a with AccC _ h => F x (fun y r => f y (h y r)) end.
-  Definition W x := W' x (alpha x).
+  Definition wf := forall x, Acc x.
 End Acc.
 Arguments Acc {X}.
 Arguments W' {X R p}.
 Arguments wf {X}.
-Arguments W {X R} alpha {p}.
+Definition W {X R p} H F x := @W' X R p F x (H x).
 
-(** Successor relation is well-founded *)
+Fact lt_wf :
+  wf lt.
+Proof.
+  hnf.
+  enough (forall n x, x < n -> Acc lt x) by eauto.
+  induction n as [|n IH].
+  - easy.
+  - intros x H. constructor. intros y H1. apply IH. lia.
+Qed.
 
-Module Successor.
-  Definition SR (y x: nat) := S y = x.
-  Goal forall x, Acc SR x.
+Section Lexical_product.
+  Variables (X: Type) (R: X -> X -> Prop).
+  Variables (Y: Type) (S: Y -> Y -> Prop).
+  Definition lex (a b: X * Y) : Prop :=
+    R (fst a) (fst b) \/ fst a = fst b /\ S (snd a) (snd b).
+  Fact lex_wf :
+    wf R -> wf S -> wf lex.
   Proof.
-    induction x as [|x IH].
-    - constructor. unfold SR at 1. intros y [=].
-    - constructor. unfold SR at 1. intros y [= ->]. exact IH.
+    intros H1 H2 [x y]. revert x y.
+    refine (W H1 _). intros x IH1.
+    refine (W H2 _). intros y IH2.
+    constructor. intros [x' y']. unfold lex at 1. cbn. intros [H|[-> H]].
+    - apply IH1, H.
+    - apply IH2, H.
   Qed.
-End Successor.
+End Lexical_product.
 
-(** Transitive closure preserves well-foundedness *)
+Section Retract.
+  Variables (X Y: Type) (R: Y -> Y -> Prop) (sigma: X -> Y).
+  Definition retract (x x': X) := R (sigma x) (sigma x').
+  Lemma retract_Acc :
+    forall x, Acc R (sigma x) -> Acc retract x.
+  Proof.
+    enough (forall y, Acc R y -> forall x, y = sigma x -> Acc retract x) by eauto.
+    refine (W' _). intros y IH x ->.
+    constructor. unfold retract at 1. intros y H.
+    eapply IH. exact H. reflexivity.
+  Qed.
+        
+  Fact retract_wf :
+    wf R -> wf retract.
+  Proof.
+    intros H x. apply retract_Acc, H.
+  Qed.
+End Retract.
 
-Section TC.
+Section Transitive_closure.
   Variables (X: Type) (R: X -> X -> Prop).
   Inductive TC (x y: X) : Prop :=
   | TC1 : R x y -> TC x y
   | TC2 y' :TC x y' -> R y' y -> TC x y.
-  Goal wf R -> wf TC.
+  Fact TC_wf :
+    wf R -> wf TC.
   Proof.
     intros H. hnf.
     refine (W H _). intros y IH.
@@ -47,6 +85,64 @@ Section TC.
     - apply IH in H2. destruct H2 as [H2].
       apply H2, H1.
   Qed.                               
-End TC.
+End Transitive_closure.
 
-(** Exercise: Prove that (TC SR) is < on numbers *)
+Section Successor_relation.
+  Definition R_S (x y: nat) := S x = y.
+  Fact R_S_wf :
+    wf R_S.
+  Proof.
+    hnf. induction x as [|x IH].
+    - constructor. unfold R_S at 1. easy.
+    - constructor. unfold R_S at 1. intros y [= ->]. exact IH.
+  Qed.
+End Successor_relation.
+
+(** Exercise: Prove that (TC R_S) is < on numbers *)
+
+From Coq Require Import Classical_Prop FunctionalExtensionality.
+
+Fact Acc_pure X (R: X -> X -> Prop) :
+  forall x (a a': Acc R x), a = a'.
+Proof.
+  enough (forall x (a: Acc R x) (a a': Acc R x), a = a') by eauto.
+  refine (W' _). intros x IH [h] [h']. f_equal.
+  extensionality y. extensionality r. apply IH, r.
+Qed.
+
+Print Assumptions Acc_pure.
+
+Section Unfolding_equation.
+  Variables (X: Type) (R: X -> X -> Prop) (R_wf: wf R).
+  Variable p: X -> Type.
+  Variables F: forall x, (forall y, R y x -> p y) -> p x.
+  Fact W_eq x :
+    W R_wf F x = F x (fun y _ => W R_wf F y).
+  Proof.
+    unfold W. destruct (R_wf x) as [h]. cbn.
+    f_equal. extensionality y. extensionality r.
+    f_equal. apply Acc_pure.
+  Qed.
+End Unfolding_equation.
+Arguments W_eq {X R R_wf p F}.
+
+Section Div.
+  Variable y: nat.
+  Implicit Types (x: nat) (g: nat -> nat).
+  (* Unguarded step function *)
+  Definition G g x : nat :=
+    if le_lt_dec x y then 0 else S (g (x - S y)).
+  (* Guarded step function *)
+  Definition F x (h: forall x', x' < x -> nat) : nat.
+    refine (if le_lt_dec x y then 0 else S (h (x - S y) _)).
+    abstract lia. 
+  Defined.
+  Definition g: nat -> nat := W lt_wf F.
+
+  Fact g_eq :
+    forall x, g x = if le_lt_dec x y then 0 else S (g (x - S y)).
+  Proof.
+    exact W_eq.
+  Qed.
+End Div.
+
